theories/examples/enclaves/trusted_compute_adequacy.v
@@ -1,0 +1,154 @@
+(* From iris.algebra Require Import frac. *)
+(* From iris.proofmode Require Import proofmode. *)
+(* Require Import Eqdep_dec List. *)
+(* From cap_machine Require Import rules seal_store. *)
+(* From cap_machine Require Import logrel fundamental. *)
+(* From cap_machine Require Import proofmode. *)
+(* From cap_machine Require Import macros_new. *)
+(* Open Scope Z_scope. *)
+From iris.proofmode Require Import proofmode.
+From cap_machine Require Import rules logrel fundamental.
+From cap_machine Require Import proofmode.
+From cap_machine Require Import assert macros_new.
+From cap_machine Require Import
+  trusted_compute_code
+  trusted_compute_enclave_spec
+  trusted_compute_spec
+.
+(* From cap_machine Require Import attestation_adequacy_template. *)
+
+(* Instance DisjointList_list_Addr : DisjointList (list Addr). *)
+(* Proof. exact (@disjoint_list_default _ _ app []). Defined. *)
+
+Class memory_layout `{MachineParameters} := {
+  (* Verifier code *)
+  verifier_region_start : Addr;
+  verifier_start : Addr;
+  verifier_end : Addr;
+  verifier_size: (verifier_start + trusted_compute_main_len = Some verifier_end)%a;
+  verifier_region_start_offset: (verifier_region_start + 0)%a = Some verifier_start;
+  verifier_region: list Addr;
+  verifier_region_correct:
+    verifier_region = (finz.seq_between verifier_region_start verifier_end);
+
+  (* Adversary code *)
+  adv_region_start : Addr;
+  adv_start : Addr;
+  adv_end : Addr;
+  adv_instrs : list Word;
+  adv_size : (adv_start + (length adv_instrs) = Some adv_end)%a ;
+  adv_region_start_offset: (adv_region_start + 0)%a = Some adv_start;
+  adv_region: list Addr;
+  adv_region_correct:
+    adv_region = (finz.seq_between adv_region_start adv_end);
+
+  (* Assert routine *)
+  l_assert_start : Addr;
+  l_assert_cap : Addr;
+  l_assert_flag : Addr;
+  l_assert_end : Addr;
+
+  l_assert_code_size :
+    (l_assert_start + length assert_subroutine_instrs)%a = Some l_assert_cap;
+  l_assert_cap_size :
+    (l_assert_cap + 1)%a = Some l_assert_flag;
+  l_assert_flag_size :
+    (l_assert_flag + 1)%a = Some l_assert_end;
+  l_assert_region: list Addr;
+  l_assert_region_correct:
+    l_assert_region = (finz.seq_between l_assert_start l_assert_end);
+
+  (* link table *)
+  link_table_start : Addr;
+  link_table_end : Addr;
+
+  link_table_size :
+    (link_table_start + 1)%a = Some link_table_end;
+  link_table_region: list Addr;
+  link_table_region_correct:
+    link_table_region = (finz.seq_between l_assert_start l_assert_end);
+
+  regions_disjoints :
+  verifier_region ## adv_region ∧
+  verifier_region ## l_assert_region ∧
+  verifier_region ## link_table_region ∧
+  adv_region ## l_assert_region ∧
+  adv_region ## link_table_region ∧
+  l_assert_region ## link_table_region;
+}.
+
+(* Definition tc_verifier_prog `{memory_layout} : prog := *)
+(*   {| prog_start := verifier_start ; *)
+(*      prog_end := verifier_end ; *)
+(*      prog_instrs := trusted_compute_main_code 0 ; *)
+(*      prog_size := verifier_size |}. *)
+
+(* Definition adv_prog `{memory_layout} : prog := *)
+(*   {| prog_start := adv_start ; *)
+(*      prog_end := adv_end ; *)
+(*      prog_instrs := adv_instrs ; *)
+(*      prog_size := adv_size |}. *)
+
+(* Program Definition layout `{memory_layout} : ocpl_library := *)
+(*   {| (* malloc library *) *)
+(*      malloc_start := l_malloc_start; *)
+(*      malloc_memptr := l_malloc_memptr; *)
+(*      malloc_mem_start := l_malloc_mem_start; *)
+(*      malloc_end := l_malloc_end; *)
+
+(*      malloc_code_size := l_malloc_code_size; *)
+
+(*      malloc_memptr_size := l_malloc_memptr_size; *)
+
+(*      malloc_mem_size := l_malloc_mem_size; *)
+
+(*      (* assertion fail library *) *)
+(*      assert_start := l_assert_start; *)
+(*      assert_cap := l_assert_cap; *)
+(*      assert_flag := l_assert_flag; *)
+(*      assert_end := l_assert_end; *)
+
+(*      assert_code_size := l_assert_code_size; *)
+(*      assert_cap_size := l_assert_cap_size; *)
+(*      assert_flag_size := l_assert_flag_size; *)
+
+(*      (* disjointness of the two libraries *) *)
+(*      libs_disjoint := _ *)
+(*   |}. *)
+(* Next Obligation. *)
+(*   intros. *)
+(*   pose proof (regions_disjoint) as Hdisjoint. *)
+(*   rewrite !disjoint_list_cons in Hdisjoint |- *. *)
+(*   set_solver. *)
+(* Qed. *)
+(* Definition OCPLLibrary `{memory_layout} := library layout. *)
+
+(* Program Definition roe_table `{memory_layout} : @tbl_priv roe_prog OCPLLibrary := *)
+(*   {| prog_lower_bound := f_region_start ; *)
+(*      tbl_start := link_table_start ; *)
+(*      tbl_end := link_table_end ; *)
+(*      tbl_size := link_table_size ; *)
+(*      tbl_prog_link := f_region_start_offset ; *)
+(*      tbl_disj := _ *)
+(*   |}. *)
+(* Next Obligation. *)
+(*   intros. simpl. *)
+(*   pose proof (regions_disjoint) as Hdisjoint. *)
+(*   rewrite !disjoint_list_cons in Hdisjoint |- *. *)
+(*   disjoint_map_to_list. set_solver. *)
+(* Qed. *)
+
+(* Program Definition adv_table `{memory_layout} : @tbl_pub adv_prog OCPLLibrary := *)
+(*   {| prog_lower_bound := adv_region_start ; *)
+(*      tbl_start := adv_link_table_start ; *)
+(*      tbl_end := adv_link_table_end ; *)
+(*      tbl_size := adv_link_table_size ; *)
+(*      tbl_prog_link := adv_region_start_offset ; *)
+(*      tbl_disj := _ *)
+(*   |}. *)
+(* Next Obligation. *)
+(*   intros. simpl. *)
+(*   pose proof (regions_disjoint) as Hdisjoint. *)
+(*   rewrite !disjoint_list_cons in Hdisjoint |- *. *)
+(*   disjoint_map_to_list. set_solver. *)
+(* Qed. *)
