theories/examples/enclaves/trusted_compute_code.v
@@ -1,0 +1,184 @@
+From iris.proofmode Require Import proofmode.
+From cap_machine Require Import logrel proofmode.
+From cap_machine Require Import macros_new hash_cap.
+
+Class TrustedCompute := {
+    tc_addr : Addr;
+  }.
+
+Section trusted_example.
+  Context {Σ:gFunctors} {ceriseg:ceriseG Σ} {sealsg : sealStoreG Σ}
+    `{reservedaddresses : ReservedAddresses}
+    {nainv: logrel_na_invs Σ} `{MP: MachineParameters}.
+  Context {TC : TrustedCompute}.
+
+  (* --------------------------------- *)
+  (* --- TRUSTED COMPUTE *ENCLAVE* --- *)
+  (* --------------------------------- *)
+
+  Definition trusted_compute_enclave_instrs : list instr :=
+    [
+      (* get signing sealing key *)
+      Mov r_t1 PC;
+      Lea r_t1 (-1)%Z;
+      Load r_t1 r_t1;
+      GetB r_t2 r_t1;
+      GetA r_t3 r_t1;
+      Sub r_t2 r_t2 r_t3;
+      Lea r_t1 r_t2;
+      Load r_t1 r_t1;
+      GetE r_t3 r_t1;
+      Sub r_t2 r_t3 1;
+      Subseg r_t1 r_t2 r_t3;
+
+      (* store the result (42) in a O-permission capability and sign it *)
+      Mov r_t2 PC;
+      GetA r_t3 r_t2;
+      Sub r_t3 42 r_t3;
+      Lea r_t2 r_t3;
+      Restrict r_t2 (encodePerm O);
+      Lea r_t1 1;
+      Seal r_t2 r_t1 r_t2;
+
+      (* share the signed value and the unsealing key to the adversary *)
+      Restrict r_t1 (encodeSealPerms (false, true)); (* restrict r1 U *)
+      Jmp r_t0
+    ].
+  Definition trusted_compute_enclave_code : list Word :=
+    encodeInstrsW trusted_compute_enclave_instrs.
+
+  Definition trusted_compute_enclave_lcode : list LWord :=
+    encodeInstrsLW trusted_compute_enclave_instrs.
+
+  Definition hash_trusted_compute_enclave : Z :=
+    hash_concat (hash tc_addr) (hash trusted_compute_enclave_code).
+
+
+  (* ---------------------------------- *)
+  (* ----- TRUSTED COMPUTE *MAIN* ----- *)
+  (* ---------------------------------- *)
+
+  Definition trusted_compute_main_code_init0 (main callback data : Z) : list LWord :=
+    (* main: *)
+    encodeInstrsLW [
+        Mov r_t1 PC;      (* rt1 := (RWX, main, main_end, main) *)
+
+        (* Create callback sentry *)
+        Lea r_t1 (callback - main)%Z;       (* rt1 := (RWX, main, main_end, callback) *)
+        Restrict r_t1 (encodePerm E);       (* rt1 := (E, main, main_end, callback) *)
+
+        (* Jump to adversary *)
+        Jmp r_t0
+      ].
+
+  (* Expect PC := (RWX, main, main_end, callback) *)
+  Definition trusted_compute_main_code_callback0
+    (callback fails : Z)
+    (hash_enclave : Z)
+    (assert_lt_offset : Z)
+    : list LWord :=
+      (* callback: *)
+      encodeInstrsLW [
+        (* until the end, r3 contains the capability that bails out if something is wrong *)
+        Mov r_t3 PC ;                 (* r_t3 :=  (RX, main, main_end, callback) *)
+        Mov r_t4 r_t3 ;               (* r_t4 :=  (RX, main, main_end, callback) *)
+        Lea r_t3 (fails-callback)%Z;  (* r_t3 :=  (RX, main, main_end, fails) *)
+
+        (* sanity check: w_res is a sealed capability *)
+        GetOType r_t2 r_t0;
+        Sub r_t2 r_t2 (-1)%Z;
+        Mov r_t5 PC ;
+        Lea r_t5 4 ;
+        Jnz r_t5 r_t2;
+        Jmp r_t3;
+
+        (*  attestation *)
+        GetOType r_t2 r_t0;
+        EStoreId r_t4 r_t2;
+        (* check otype(w_res) against identity of the enclave *)
+        Sub r_t4 r_t4 hash_enclave;
+        Jnz r_t3 r_t4;
+
+        (* get returned value and assert it to be 42 *)
+        UnSeal r_t1 r_t1 r_t0;
+        Mov r_t0 r_t5;
+        GetA r_t4 r_t1;
+        Mov r_t5 42%Z;
+        Mov r_t1 r_t3%Z;
+        Lea r_t1 1;
+        Load r_t1 r_t1
+      ]
+      ++ assert_reg_instrs assert_lt_offset r_t1
+      ++ encodeInstrsLW [Mov r_t0 0 ; Mov r_t3 0 ; Halt]
+      ++ (* fails: *) encodeInstrsLW [Fail].
+
+  Definition trusted_compute_main_init_len : Z :=
+    Eval cbv in (length (trusted_compute_main_code_init0 0%Z 0%Z 0%Z)).
+
+  Definition trusted_compute_main_callback_len : Z :=
+    Eval cbv in (length (trusted_compute_main_code_callback0 0%Z 0%Z 0%Z 0%Z)).
+
+  Definition trusted_compute_main_code (assert_lt_offset : Z) : list LWord :=
+    let init     := 0%Z in
+    let callback := trusted_compute_main_init_len in
+    let data     := (trusted_compute_main_init_len + trusted_compute_main_callback_len)%Z in
+    let fails    := (data - 1)%Z in
+    (trusted_compute_main_code_init0 init callback data) ++
+    (trusted_compute_main_code_callback0 callback fails hash_trusted_compute_enclave assert_lt_offset).
+
+  Definition trusted_compute_main_code_len : Z :=
+    Eval cbv in trusted_compute_main_init_len + trusted_compute_main_callback_len.
+
+  Definition trusted_compute_main_data_len : Z := 2.
+  Definition trusted_compute_main_len :=
+    Eval cbv in (trusted_compute_main_code_len + trusted_compute_main_data_len)%Z.
+
+
+  (* Sealed predicate for TC enclave *)
+
+  Program Definition f42 : Addr := (finz.FinZ 42 eq_refl eq_refl).
+  Definition sealed_42 : LWord → iProp Σ :=
+    λ w, (∃ b e v, ⌜w = LCap O b e f42 v⌝)%I.
+  Definition sealed_42_ne : (leibnizO LWord) -n> (iPropO Σ) :=
+      λne (w : leibnizO LWord), sealed_42 w%I.
+
+  Instance sealed_42_persistent w : Persistent (sealed_42 w).
+  Proof. apply _. Qed.
+
+  Definition seal_pred_42 τ := seal_pred τ sealed_42.
+  Definition valid_sealed_cap w τ := valid_sealed w τ sealed_42.
+  Lemma sealed_42_interp lw : sealed_42 lw -∗ fixpoint interp1 lw.
+  Proof.
+    iIntros "Hsealed". iDestruct "Hsealed" as (b e v) "->".
+    by rewrite fixpoint_interp1_eq /=.
+  Qed.
+
+  (* TC Custom Predicates *)
+  Definition tc_enclave_pred : CustomEnclave :=
+    @MkCustomEnclave Σ
+      trusted_compute_enclave_code
+      tc_addr
+      (λ w, False%I)
+      sealed_42.
+
+  Definition tcenclaves_map : custom_enclaves_map :=
+   {[hash_trusted_compute_enclave := tc_enclave_pred]}.
+
+  Lemma wf_tc_enclaves_map :
+    custom_enclaves_map_wf tcenclaves_map.
+  Proof.
+    rewrite /custom_enclaves_map_wf /tcenclaves_map.
+    split.
+    - by rewrite map_Forall_singleton /hash_trusted_compute_enclave /=.
+    - rewrite map_Forall_singleton; cbn.
+      rewrite /encodeInstrW.
+      apply Forall_forall.
+      intros w Hw.
+      repeat (rewrite elem_of_cons in Hw ; destruct Hw as [-> | Hw]; first done).
+      by rewrite elem_of_nil in Hw.
+  Qed.
+
+  Definition contract_tc_enclaves_map :=
+    MkCustomEnclavesMap tcenclaves_map wf_tc_enclaves_map.
+
+End trusted_example.
