theories/examples/enclaves/trusted_compute_enclave_spec.v
@@ -1,0 +1,256 @@
+From iris.proofmode Require Import proofmode.
+From cap_machine Require Import rules logrel fundamental.
+From cap_machine Require Import proofmode.
+From cap_machine Require Import trusted_compute_code.
+Open Scope Z_scope.
+
+
+Section trusted_compute_enclave.
+  Context {Σ:gFunctors} {ceriseg:ceriseG Σ} {sealsg: sealStoreG Σ}
+          {nainv: logrel_na_invs Σ}
+          {reservedaddresses : ReservedAddresses}
+          `{MP: MachineParameters}.
+  Context {TC : TrustedCompute}.
+
+  Lemma tc_enclave_contract :
+    ⊢ custom_enclave_contract (enclaves_map := contract_tc_enclaves_map).
+  Proof.
+    iLöb as "IH".
+    rewrite -/custom_enclave_contract.
+    iEval (rewrite /custom_enclave_contract).
+    iIntros (I b e v b' e' a' v' enclave_data ot ce
+      Hcode_ce Hot HIhash Hb He)
+      "(#Hcustoms_inv & #Htc_inv & #HPenc & #HPsign)".
+    assert (e = (b ^+ (length (code ce) + 1))%a) as -> by solve_addr+He.
+    simplify_map_eq.
+    rewrite /tcenclaves_map in Hcode_ce.
+    replace ((λ w : Word, word_to_lword w v) <$> code ce) with trusted_compute_enclave_lcode.
+    2:{ simplify_map_eq. cbn. rewrite /encodeInstrWL. done. }
+    simplify_map_eq.
+    rewrite -H; clear H.
+    rewrite fixpoint_interp1_eq /=.
+    iIntros (lregs); iNext ; iModIntro.
+    iIntros "([%Hfullmap #Hinterp_map] & Hrmap & Hna)".
+    rewrite /interp_conf.
+    iMod (na_inv_acc with "Htc_inv Hna") as "(>[Htc_code Htc_data]  & Hna & Hclose)"; [solve_ndisj ..|].
+    rewrite /registers_mapsto.
+    iExtract "Hrmap" PC as "HPC".
+    remember tc_addr as pc_b in |- * at 7.
+    remember (tc_addr ^+ (20%nat + 1))%a as pc_e in |- * at 4.
+    assert (SubBounds pc_b pc_e tc_addr (tc_addr ^+ (20%nat + 1))%a) by (subst; solve_addr).
+
+    (* Prepare the necessary resources *)
+    (* Registers *)
+    assert (exists w0, lregs !! r_t0 = Some w0) as Hrt0 by apply (Hfullmap r_t0).
+    destruct Hrt0 as [w0 Hr0].
+    replace (delete PC lregs)
+            with (<[r_t0:=w0]> (delete PC lregs)).
+    2: { rewrite insert_id; auto. rewrite lookup_delete_ne; auto. }
+
+    assert (exists w1, lregs !! r_t1 = Some w1) as Hrt1 by apply (Hfullmap r_t1).
+    destruct Hrt1 as [w1 Hr1].
+    replace (delete PC lregs)
+            with (<[r_t1:=w1]> (delete PC lregs)).
+    2: { rewrite insert_id; auto. rewrite lookup_delete_ne; auto. }
+
+    assert (exists w2, lregs !! r_t2 = Some w2) as Hrt2 by apply (Hfullmap r_t2).
+    destruct Hrt2 as [w2 Hr2].
+    replace (delete PC lregs)
+            with (<[r_t2:=w2]> (delete PC lregs)).
+    2: { rewrite insert_id; auto. rewrite lookup_delete_ne; auto. }
+
+    assert (exists w3, lregs !! r_t3 = Some w3) as Hrt3 by apply (Hfullmap r_t3).
+    destruct Hrt3 as [w3 Hr3].
+    replace (delete PC lregs)
+            with (<[r_t3:=w3]> (delete PC lregs)).
+    2: { rewrite insert_id; auto. rewrite lookup_delete_ne; auto. }
+
+    (* EXTRACT REGISTERS FROM RMAP *)
+    (* iExtractList "Hrmap" [r_t0;r_t1;r_t2;r_t3] as ["Hr0";"Hr1";"Hr2";"Hr3"]. *)
+    iDestruct (big_sepM_delete _ _ r_t0 with "Hrmap") as "[Hr0 Hrmap]".
+    { by simplify_map_eq. }
+    iDestruct (big_sepM_delete _ _ r_t1 with "Hrmap") as "[Hr1 Hrmap]".
+    { by simplify_map_eq. }
+    iDestruct (big_sepM_delete _ _ r_t2 with "Hrmap") as "[Hr2 Hrmap]".
+    { by simplify_map_eq. }
+    iDestruct (big_sepM_delete _ _ r_t3 with "Hrmap") as "[Hr3 Hrmap]".
+    { by simplify_map_eq. }
+    replace (delete r_t3 _) with
+      ( delete r_t3 (delete r_t2 (delete r_t1 (delete r_t0 (delete PC lregs))))).
+    2:{
+      rewrite delete_insert_delete; repeat rewrite (delete_insert_ne _ r_t0) //.
+      rewrite delete_insert_delete; repeat rewrite (delete_insert_ne _ r_t1) //.
+      rewrite delete_insert_delete; repeat rewrite (delete_insert_ne _ r_t2) //.
+      rewrite delete_insert_delete; repeat rewrite (delete_insert_ne _ r_t3) //.
+      done.
+    }
+    (* Code memory *)
+    iDestruct (region_mapsto_cons with "Htc_code") as "[Htc_addr Htc_code]"; last iFrame.
+    { transitivity (Some (tc_addr ^+ 1)%a); auto ; try solve_addr. }
+    { solve_addr. }
+    iAssert (codefrag (tc_addr ^+ 1%nat)%a v trusted_compute_enclave_lcode)
+      with "[Htc_code]" as "Htc_code".
+    {
+      rewrite /codefrag /=.
+      by replace ((tc_addr ^+ 1%nat) ^+ 20%nat)%a with (tc_addr ^+ 21%nat)%a by solve_addr.
+    }
+    codefrag_facts "Htc_code".
+
+    (* Data memory *)
+    iAssert (⌜ (b' < e')%a ⌝)%I as "%Hb'".
+    {
+      iDestruct (big_sepL2_length with "Htc_data") as "%Htc_data_len".
+      rewrite map_length /= in Htc_data_len.
+      iPureIntro.
+      clear - Htc_data_len.
+      destruct (decide (b' < e')) as [He' | He']; cycle 1.
+      - rewrite finz_seq_between_empty in Htc_data_len; last solve_addr.
+        cbn in * ; discriminate.
+      - done.
+    }
+    iDestruct (region_mapsto_cons with "Htc_data") as "[Htc_keys Htc_data]"; last iFrame.
+    { transitivity (Some (b' ^+ 1)%a); auto ; try solve_addr. }
+    { solve_addr. }
+
+
+    (* Prove the spec *)
+    iInstr "Htc_code". (* Mov r_t1 PC *)
+    iInstr "Htc_code". (* Lea r_t1 (-1)%Z *)
+    transitivity (Some tc_addr); auto ; solve_addr.
+
+    iInstr "Htc_code". (* Load r_t1 r_t1 *)
+    apply le_addr_withinBounds; solve_addr.
+    iInstr "Htc_code". (* GetB r_t2 r_t1 *)
+    iInstr "Htc_code". (* GetA r_t3 r_t1 *)
+    iInstr "Htc_code". (* Sub r_t2 r_t2 r_t3 *)
+    iInstr "Htc_code". (* Lea r_t1 r_t2 *)
+    transitivity (Some b'); auto ; solve_addr.
+
+    iInstr "Htc_code". (* Load r_t1 r_t1 *)
+    apply le_addr_withinBounds; solve_addr.
+    iInstr "Htc_code". (* GetE r_t3 r_t1 *)
+    iInstr "Htc_code". (* Sub r_t3 r_t2 1 *)
+    replace (((ot ^+ 2)%f - 1)) with (ot + 1) by solve_finz.
+    iInstr "Htc_code". (* Subseg r_t1 r_t2 r_t3 *)
+    transitivity (Some (ot ^+1)%ot); auto ; solve_finz.
+    apply isWithin_of_le; solve_finz.
+
+    iInstr "Htc_code". (* Mov r_t2 PC *)
+    iInstr "Htc_code". (* GetA r_t3 r_t2 *)
+    iInstr "Htc_code". (* Sub r_t3 42 r_t3 *)
+
+    assert (
+        ((tc_addr ^+ 1) ^+ 11 + (42 - ((tc_addr ^+ 1) ^+ 11)))%a = Some f42)
+      as Hoffset by (by rewrite finz_incr_minus_id).
+    iInstr "Htc_code". (* Lea r_t2 r_t3 *)
+    iInstr "Htc_code". (* Restrict r_t2 (encodePerm O) *)
+    by rewrite decode_encode_perm_inv.
+    rewrite decode_encode_perm_inv.
+    iInstr "Htc_code". (* Lea r_t1 1 *)
+    transitivity (Some (ot ^+ 1)%ot); auto ; solve_finz.
+    iInstr "Htc_code". (* Seal r_t2 r_t2 r_t1 *)
+    by cbn.
+    apply le_addr_withinBounds; solve_finz.
+
+    (* Restrict r_t1 (encodeSealPerms (false, true)) *)
+    iInstr_lookup "Htc_code" as "Hi" "Htc_code".
+    wp_instr.
+    iApply (wp_restrict_success_z_sr with "[HPC Hr1 Hi]")
+    ; try iFrame
+    ; try solve_pure
+    ; repeat (rewrite decode_encode_seal_perms_inv)
+    ; try done.
+    iNext; iIntros "(HPC & Hi & Hr1)".
+    all: wp_pure; iInstr_close "Htc_code".
+
+    (* Prepare the jump to adversary: prove all registers contain safe values *)
+    iAssert (interp w0) as "Hinterp_w0".
+    { iApply "Hinterp_map" ; eauto; done. }
+
+    iAssert (interp (LSealedCap (ot ^+ 1)%f O tc_addr (tc_addr ^+ 21%nat)%a f42 v))
+      as "Hinterp_sealed42".
+    {
+      iClear "Hinterp_map Hinterp_w0".
+      rewrite /= fixpoint_interp1_eq /= /interp_sb.
+      iExists sealed_42; iFrame "%#".
+      iSplit.
+      { iPureIntro; intro; apply sealed_42_persistent. }
+      { iNext; by iExists _,_,_. }
+    }
+
+    iAssert (interp (LSealRange (false, true) (ot ^+ 1)%f (ot ^+ 2)%f (ot ^+ 1)%f))
+      as "Hinterp_sign".
+    {
+      iClear "Hinterp_map Hinterp_w0 Hinterp_sealed42".
+      rewrite /= fixpoint_interp1_eq /= /safe_to_unseal.
+      iSplit ; first done.
+      rewrite finz_seq_between_singleton; cbn ; last solve_finz.
+      iSplit ; last done.
+      iSplit ; last done.
+      iExists sealed_42_ne; iFrame "#".
+      iNext ; iModIntro; iIntros (lw) "Hlw".
+      by iApply sealed_42_interp.
+    }
+
+    iDestruct (jmp_to_unknown with "[] [$Hinterp_w0]") as "Hjmp"; eauto.
+    {
+      iSplit; last iFrame "#".
+      iModIntro.
+      by iApply custom_enclave_contract_inv.
+    }
+    iInstr "Htc_code". (* Jmp r_t0 *)
+
+    (* Close the opened invariant *)
+    iDestruct (region_mapsto_cons with "[Htc_addr Htc_code]") as "Htc_code"
+    ; try iFrame
+    ; try solve_addr.
+    iDestruct (region_mapsto_cons with "[Htc_keys Htc_data]") as "Htc_data"
+    ; try iFrame
+    ; try solve_addr.
+    replace ((tc_addr ^+ 1%nat)%a ^+ length trusted_compute_enclave_lcode)%a with
+      (tc_addr ^+ 21%nat)%a by solve_addr.
+    iMod ("Hclose" with "[$Hna $Htc_code $Htc_data]") as "Hna".
+    (* Wrap up the registers *)
+    (* iInsertList "Hrmap" [r_t0;r_t1;r_t2;r_t3]. *)
+    iDestruct (big_sepM_insert _ _ r_t0 with "[$Hrmap $Hr0]") as "Hrmap".
+    { do 3 ( rewrite lookup_delete_ne //) ; by rewrite lookup_delete. }
+    do 3 (rewrite -delete_insert_ne //=); rewrite insert_delete_insert.
+    iDestruct (big_sepM_insert _ _ r_t1 with "[$Hrmap $Hr1]") as "Hrmap".
+    { do 2 ( rewrite lookup_delete_ne //) ; by rewrite lookup_delete. }
+    do 2 (rewrite -delete_insert_ne //=); rewrite insert_delete_insert.
+    iDestruct (big_sepM_insert _ _ r_t2 with "[$Hrmap $Hr2]") as "Hrmap".
+    { do 1 ( rewrite lookup_delete_ne //) ; by rewrite lookup_delete. }
+    do 1 (rewrite -delete_insert_ne //=); rewrite insert_delete_insert.
+    iDestruct (big_sepM_insert _ _ r_t3 with "[$Hrmap $Hr3]") as "Hrmap".
+    { do 0 ( rewrite lookup_delete_ne //) ; by rewrite lookup_delete. }
+    do 0 (rewrite -delete_insert_ne //=); rewrite insert_delete_insert.
+
+    set ( rmap' := <[r_t3:=LInt (42 - ((tc_addr ^+ 1) ^+ 11)%a)]>
+                            (<[r_t2:=LSealedCap (ot ^+ 1)%f O tc_addr (tc_addr ^+ 21%nat)%a f42 v]>
+                               (<[r_t1:=LSealRange (false, true) (ot ^+ 1)%f (ot ^+ 2)%f (ot ^+ 1)%f]>
+                                  (<[r_t0:=w0]> (delete PC lregs))))).
+    iAssert ([∗ map] k↦y ∈ rmap', k ↦ᵣ y ∗ interp y)%I with "[Hrmap]" as "Hrmap".
+    {
+      subst rmap'.
+      subst pc_b pc_e.
+      iApply (big_sepM_sep_2 with "[Hrmap]") ; first done.
+      iApply big_sepM_insert_2; first (iApply interp_int).
+      repeat (iApply big_sepM_insert_2; first done).
+
+      iApply big_sepM_intro.
+      iIntros "!>" (r w Hrr).
+      assert (is_Some (delete PC lregs !! r)) as His_some by auto.
+      rewrite lookup_delete_is_Some in His_some.
+      destruct His_some as [Hr _].
+      rewrite lookup_delete_ne in Hrr; auto.
+      iApply ("Hinterp_map" $! r w); auto.
+    }
+    assert (dom rmap' = all_registers_s ∖ {[PC]}).
+    {
+      repeat (rewrite dom_insert_L).
+      rewrite dom_delete_L.
+      rewrite regmap_full_dom; auto.
+    }
+    iApply ("Hjmp" with "[]") ; eauto ; iFrame.
+  Qed.
+End trusted_compute_enclave.
